Impl set_hD

pulse/examples/steel/arraystructs/LList.fst
@@ -64,160 +64,217 @@ let elim_vpure
     (fun m -> pure_interp p m; reveal_emp (); intro_emp m)
 
 let ptr = option (ref' node node)
-let cells = list (Ghost.erased int & Ghost.erased ptr)
+let cells = list (int & ptr)
 
-let pts_to_llist_cons (value: Ghost.erased int) (next: Ghost.erased ptr) (tl: cells)
+let pts_to_llist_cons (value: int) (next: ptr) (tl: cells)
   (pts_to_llist:(
-    Ghost.erased ptr ->
-    l:cells{List.length l < List.length ((value, next) :: tl)} ->
+    ptr ->
+    l:Ghost.erased cells{List.length l < List.length ((value, next) :: tl)} ->
     Tot vprop))
   (p: option (ref' node node))
   (prf: squash (Some? p /\ pcm_of_ref' (Some?.v p) == node_pcm))
 : vprop
 = let r: ref node node_pcm = Some?.v p in
   (r `pts_to` mk_node (some value) (some next)) `star`
-  (next `pts_to_llist` tl)
+  (next `pts_to_llist` Ghost.hide tl)
 
-let rec pts_to_llist (p:Ghost.erased ptr) (l:cells)
+let rec pts_to_llist ([@@@smt_fallback] p:ptr) ([@@@smt_fallback] l:Ghost.erased cells)
 : Tot vprop (decreases (List.length l))
-= match l with
-  | [] -> vpure (p == none)
+= match Ghost.reveal l with
+  | [] -> vpure (p == None)
   | (value, next) :: tl ->
     vpure (Some? p /\ pcm_of_ref' (Some?.v p) == node_pcm) `vdep`
     pts_to_llist_cons value next tl pts_to_llist p
 
 let pts_to_llist_nil_eq p
-: Lemma ((p `pts_to_llist` []) == vpure (p == none))
+: Lemma ((p `pts_to_llist` []) == vpure (p == None))
   [SMTPat (p `pts_to_llist` [])]
 = ()
 
-let pts_to_llist_cons_eq (p: Ghost.erased ptr) value next tl
-: Lemma ((p `pts_to_llist` ((value, next) :: tl)) == 
+let pts_to_llist_cons_eq (p:ptr) (value:int) (next:ptr) (tl:cells)
+: Lemma ((p `pts_to_llist` Ghost.hide ((value, next) :: tl)) == 
     vpure (Some? p /\ pcm_of_ref' (Some?.v p) == node_pcm) `vdep`
     pts_to_llist_cons value next tl pts_to_llist p)
-= assert_norm ((p `pts_to_llist` ((value, next) :: tl)) == 
+= assert_norm ((p `pts_to_llist` Ghost.hide ((value, next) :: tl)) == 
+  (match Ghost.reveal (Ghost.hide ((value, next) :: tl)) with
+  | [] -> vpure (p == None)
+  | (value, next) :: tl ->
     vpure (Some? p /\ pcm_of_ref' (Some?.v p) == node_pcm) `vdep`
-    pts_to_llist_cons value next tl pts_to_llist p)
+    pts_to_llist_cons value next tl pts_to_llist p)) 
+    // TODO Why do I have to keep the match around?
 
-let pts_to_llist_cons_eq' (p: Ghost.erased ptr) value next tl prf
+let pts_to_llist_cons_eq' (p: ptr) value (next:ptr) tl prf
 : Lemma (pts_to_llist_cons value next tl pts_to_llist p prf ==
     (let r: ref node node_pcm = Some?.v p in
-     (r `pts_to` mk_node (some value) (some next)) `star`
-     (next `pts_to_llist` tl)))
+     (r `pts_to` mk_node (some (Ghost.hide value)) (some (Ghost.hide next))) `star`
+     (next `pts_to_llist` Ghost.hide tl)))
 = assert_norm (pts_to_llist_cons value next tl pts_to_llist p prf ==
     (let r: ref node node_pcm = Some?.v p in
      (r `pts_to` mk_node (some value) (some next)) `star`
-     (next `pts_to_llist` tl)))
+     (next `pts_to_llist` Ghost.hide tl)))
 
-assume val intro_llist_nil : unit -> SteelT unit emp (fun _ -> none `pts_to_llist` [])
+val intro_llist_nil : unit -> SteelT unit emp (fun _ -> None `pts_to_llist` [])
 
-// let intro_llist_nil () =
-//   intro_vpure (none #(ref' node node) == none);
-//   pts_to_llist_nil_eq none;
-//   change_equal_slprop _ (none `pts_to_llist` [])
+let intro_llist_nil () =
+  intro_vpure (None #(ref' node node) == None);
+  pts_to_llist_nil_eq None;
+  change_equal_slprop _ (None `pts_to_llist` [])
   
-assume val intro_llist_cons
-  (#opened:inames) (r: Ghost.erased (ref node node_pcm))
-  (value: Ghost.erased int) (next: Ghost.erased ptr)
+val intro_llist_cons
+  (#opened:inames) (r: ref node node_pcm)
+  (value: int) (next: ptr)
   (tl: cells)
 : SteelGhostT unit opened
-    (r `pts_to` (mk_node (some value) (some next)) `star` (next `pts_to_llist` tl))
-    (fun _ -> some (Ghost.hide (Ghost.reveal r)) `pts_to_llist` ((value, next)::tl))
+    ((r `pts_to` mk_node (some value) (some next)) `star` (next `pts_to_llist` tl))
+    (fun _ -> Some r `pts_to_llist` ((value, next)::tl))
   
-// let intro_llist_cons r value next tl = 
-//   let p: Ghost.erased ptr = some (Ghost.hide (Ghost.reveal r)) in
-//   intro_vpure (Some? p /\ pcm_of_ref' (Some?.v p) == node_pcm);
-//   intro_vdep (vpure (Some? p /\ pcm_of_ref' (Some?.v p) == node_pcm))
-//     (r `pts_to` (mk_node (some value) (some next)) `star`
-//      (next `pts_to_llist` tl))
-//     (pts_to_llist_cons value next tl pts_to_llist p);
-//   pts_to_llist_cons_eq p value next tl;
-//   change_equal_slprop _ (some (Ghost.hide (Ghost.reveal r)) `pts_to_llist` ((value, next)::tl))
+let intro_llist_cons r value next tl = 
+  let p: ptr = Some r in
+  intro_vpure (Some? p /\ pcm_of_ref' (Some?.v p) == node_pcm);
+  intro_vdep (vpure (Some? p /\ pcm_of_ref' (Some?.v p) == node_pcm))
+    (r `pts_to` (mk_node (some value) (some next)) `star`
+     (next `pts_to_llist` tl))
+    (pts_to_llist_cons value next tl pts_to_llist p);
+  pts_to_llist_cons_eq p value next tl;
+  change_equal_slprop _ (Some r `pts_to_llist` ((value, next)::tl))
 
-assume val elim_llist_cons
-  (#opened:inames) (p: Ghost.erased ptr)
-  (value: Ghost.erased int) (next: Ghost.erased ptr)
-  (tl: cells)
+val elim_llist_cons
+  (#opened:inames) (p: ptr)
+  (value: int) (next: ptr) (tl: cells)
 : SteelGhost (Ghost.erased (ref node node_pcm)) opened
     (p `pts_to_llist` ((value, next)::tl))
     (fun r ->
       (r `pts_to` mk_node (some value) (some next)) `star`
       (next `pts_to_llist` tl))
     (requires fun _ -> True)
-    (ensures fun _ r _ -> p == some (Ghost.hide (Ghost.reveal r)))
+    (ensures fun _ r _ -> p == Some (Ghost.reveal r))
 
-// let elim_llist_cons p value next tl =
-//   pts_to_llist_cons_eq p value next tl;
-//   change_equal_slprop
-//     (p `pts_to_llist` _)
-//     (vpure (Some? p /\ pcm_of_ref' (Some?.v p) == node_pcm) `vdep`
-//      pts_to_llist_cons value next tl pts_to_llist p);
-//   let prf: Ghost.erased (t_of (vpure (Some? p /\ pcm_of_ref' (Some?.v p) == node_pcm))) =
-//     elim_vdep 
-//       (vpure (Some? p /\ pcm_of_ref' (Some?.v p) == node_pcm))
-//       (pts_to_llist_cons value next tl pts_to_llist p)
-//   in
-//   elim_vpure (Some? p /\ pcm_of_ref' (Some?.v p) == node_pcm);
-//   pts_to_llist_cons_eq' p value next tl prf;
-//   let r: Ghost.erased (ref node node_pcm) = Some?.v p in
-//   change_equal_slprop
-//     (pts_to_llist_cons value next tl pts_to_llist p prf)
-//     ((Ghost.reveal r `pts_to`
-//       mk_node (some value) (some next)) `star`
-//      (next `pts_to_llist` tl));
-//   r
+let elim_llist_cons p value next tl =
+  pts_to_llist_cons_eq p value next tl;
+  change_equal_slprop
+    (p `pts_to_llist` _)
+    (vpure (Some? p /\ pcm_of_ref' (Some?.v p) == node_pcm) `vdep`
+     pts_to_llist_cons value next tl pts_to_llist p);
+  let prf: Ghost.erased (t_of (vpure (Some? p /\ pcm_of_ref' (Some?.v p) == node_pcm))) =
+    elim_vdep 
+      (vpure (Some? p /\ pcm_of_ref' (Some?.v p) == node_pcm))
+      (pts_to_llist_cons value next tl pts_to_llist p)
+  in
+  elim_vpure (Some? p /\ pcm_of_ref' (Some?.v p) == node_pcm);
+  pts_to_llist_cons_eq' p value next tl prf;
+  let r: Ghost.erased (ref node node_pcm) = Some?.v p in
+  change_equal_slprop
+    (pts_to_llist_cons value next tl pts_to_llist p prf)
+    ((Ghost.reveal r `pts_to` mk_node (some value) (some next)) `star`
+     (next `pts_to_llist` tl));
+  r
 
 let rec values (l:cells) : GTot (list int) =
   match l with
   | [] -> []
-  | (value, _)::tl -> Ghost.reveal value :: values tl
-  
-val new_llist (init:int)
-  : Steel (ptr & cells)
-          emp
-          (fun (p, l) -> p `pts_to_llist` l)
-          (requires fun _ -> True)
-          (ensures fun _ (p, l) _ -> values l == [init])
+  | (value, _) :: tl -> Ghost.reveal value :: values tl
 
 #set-options "--ide_id_info_off"
 
-let new_llist (init:int) =
-  let cell: Ghost.erased int & Ghost.erased ptr = (Ghost.hide init, Ghost.hide None) in
-  let r = ref_alloc node_pcm (mk_node_tot (Some init) (Some None)) in
-  intro_llist_nil ();
-  change_equal_slprop
-    (r `pts_to` Ghost.hide (mk_node_tot (Some init) (Some None)))
-    (Ghost.reveal (Ghost.hide r) `pts_to` mk_node (some init) (some none));
-  intro_llist_cons r (Ghost.hide init) (Ghost.hide None) [];
-  change_equal_slprop (some _ `pts_to_llist` _) (Some r `pts_to_llist` _);
-  return (Some r, [cell])
-
-val push (p:ptr) (l:cells) (value:int)
-: Steel (ptr & cells)
+val push (p:ptr) (l:Ghost.erased cells) (value:int)
+: Steel (ptr & Ghost.erased cells)
     (p `pts_to_llist` l)
     (fun (p', l') -> p' `pts_to_llist` l')
     (requires fun _ -> True)
     (ensures fun _ (_, l') _ -> values l' == value :: values l)
 
 let push p l value =
-  let cell: Ghost.erased int & Ghost.erased ptr = (Ghost.hide value, Ghost.hide p) in
+  let cell: int & ptr = (value, p) in
   let r = ref_alloc node_pcm (mk_node_tot (Some value) (Some p)) in
-  change_equal_slprop
-    (r `pts_to` Ghost.hide (mk_node_tot (Some value) (Some p)))
-    (Ghost.reveal (Ghost.hide r) `pts_to` mk_node (some value) (some (Ghost.hide p)));
-  intro_llist_cons (Ghost.hide r) (Ghost.hide value) (Ghost.hide p) l;
-  change_equal_slprop (some _ `pts_to_llist` _) (Some r `pts_to_llist` _);
-  return (Some r, cell :: l)
+  intro_llist_cons r value p l;
+  return (Some r, Ghost.hide (cell :: l))
+  
+let cells_set_hd x (l: cells) = match l with
+  | [] -> []
+  | (_, next) :: l' -> (x, next) :: l'
 
-//val ref_alloc
-//  (#a:Type0) (p: pcm a) (x: a)
-//: Steel (ref a p)
-//    emp
-//    (fun r -> r `pts_to` x)
-//    (requires fun _ -> p_refine p x)
-//    (ensures fun _ _ _ -> True)
+/// Mutate the head of a list
 
-//elim_vdep
+// TODO does this exist already?
+assume val exfalso (#opened:inames) (p:vprop) (q:prop)
+: SteelGhost unit opened emp (fun _ -> p) (requires fun _ -> False) (ensures fun _ _ _ -> q)
+
+val pts_to_llist_nullptr (#opened:inames) (p:ptr) (l:Ghost.erased cells)
+: SteelGhost unit opened
+    (p `pts_to_llist` l) 
+    (fun _ -> None `pts_to_llist` [])
+    (requires fun _ -> p == None)
+    (ensures fun _ _ _ -> Ghost.reveal l == [])
+
+let pts_to_llist_nullptr p l =
+  match Ghost.reveal l with
+  | [] -> change_equal_slprop (p `pts_to_llist` l) (None `pts_to_llist` [])
+  | (value, next) :: tl ->
+    change_equal_slprop (p `pts_to_llist` l) (None `pts_to_llist` ((value, next) :: tl));
+    let r = elim_llist_cons None value next tl in
+    assert (None == Some r);
+    sladmit() // TODO
+    //exfalso (None `pts_to_llist` []) (Ghost.reveal l == [])
+
+[@@erasable]
+noeq type pts_to_llist_res = {
+  value: int;
+  next: ptr;
+  tl: cells;
+}
+
+val pts_to_llist_some (#opened:inames) (p:ptr) (l:Ghost.erased cells)
+: SteelGhost pts_to_llist_res opened
+    (p `pts_to_llist` l) 
+    (fun res -> p `pts_to_llist` ((res.value, res.next) :: res.tl))
+    (requires fun _ -> Some? p)
+    (ensures fun _ res _ ->
+      Some? p /\ pcm_of_ref' (Some?.v p) == node_pcm /\
+      Ghost.reveal l == ((res.value, res.next) :: res.tl))
+
+let pts_to_llist_some p l =
+  match Ghost.reveal l with
+  | [] ->
+    change_equal_slprop (p `pts_to_llist` l) (p `pts_to_llist` []);
+    assert (Some? p /\ p == None);
+    sladmit() // TODO
+  | (value, next) :: tl ->
+    change_equal_slprop (p `pts_to_llist` l) (p `pts_to_llist` ((value, next) :: tl));
+    {value; next; tl}
+
+val set_hd (p:ptr) (l:cells) (value:int)
+: SteelT unit
+    (p `pts_to_llist` l)
+    (fun _ -> p `pts_to_llist` cells_set_hd value l)
+
+let set_hd p l new_value =
+  match p with
+  | None -> pts_to_llist_nullptr p l; return ()
+  | Some r ->
+    let res = pts_to_llist_some p l in
+    let value: Ghost.erased int = Ghost.hide res.value in
+    let next: Ghost.erased ptr = Ghost.hide res.next in
+    let tl: Ghost.erased cells = Ghost.hide res.tl in
+    //let value: Ghost.erased int = Ghost.hide (fst value_next_tl) in
+    //let next: Ghost.erased ptr = Ghost.hide (fst (snd value_next_tl)) in
+    //let tl: Ghost.erased cells = Ghost.hide (snd (snd value_next_tl)) in
+    change_equal_slprop (p `pts_to_llist` l)
+      (Some r `pts_to_llist`
+       Ghost.hide ((Ghost.reveal value, Ghost.reveal next) :: Ghost.reveal tl));
+    let r' = elim_llist_cons (Some r) (Ghost.reveal value) (Ghost.reveal next) (Ghost.reveal tl) in
+    let r: ref node node_pcm = r in
+    //assert (Ghost.reveal r' == r);
+    //slassert (Ghost.reveal r' `pts_to` mk_node (some value) (some next));
+    change_equal_slprop (Ghost.reveal r' `pts_to` mk_node (some value) (some next))
+      (r `pts_to` mk_node (some value) (some next));
+    let r_value = addr_of_value r in
+    r_value `opt_write` new_value;
+    unaddr_of_value r r_value;
+    intro_llist_cons r new_value next tl;
+    //change_equal_slprop (Ghost.reveal r' `pts_to` mk_node _ _) (r `pts_to` mk_node _ _);
+    //sladmit(); return ()
+    return ()
+
 // Mutate the kth element of a list (of fixed k)
 // 
 // t k = type of functions that mutate kth element of a list
@@ -228,21 +285,7 @@ let push p l value =
 // let rec set k .. : Steel _ = 
 // let rec set k .. : Tot (.. -> Steel _) = 
 
-val push (#a:Type) (ptr:t a) (l:list (cell a)) (v:a)
-  : Steel (t a & list (cell a))
-          (llist ptr l)
-          (fun pc -> llist (fst pc) (snd pc))
-          (requires fun _ -> True)
-          (ensures fun _ pc _ -> datas (snd pc) == v::datas l)
-
-let push #a ptr l v =
-  let cell = mk_cell ptr v in
-  let p = alloc_pt cell in
-  rewrite_slprop (llist ptr l) (llist (next cell) l) (fun _ -> ());
-  intro_llist_cons p cell l;
-  let pc = p, (cell::l) in
-  pc
-
+(*
 val pop (#a:Type) (ptr:t a) (l:list (cell a){Cons? l})
   : Steel a
           (llist ptr l)
@@ -260,3 +303,4 @@ let pop #a ptr l =
   free_pt ptr;
   rewrite_slprop (llist (next hd) tl) (llist (next (L.hd l)) (L.tl l)) (fun _ -> ());
   return (data c)
+*)
